Move MerkleTrees in trees.

src/dafny/smart/DepositSmart.dfy
@@ -20,12 +20,12 @@ include "./paths/PathInCompleteTrees.dfy"
 include "./paths/NextPathInCompleteTreesLemmas.dfy"
 include "./seqofbits/SeqOfBits.dfy"
 include "./trees/Trees.dfy"
-include "./MerkleTrees.dfy"
-include "./intdiffalgo/IndexBasedAlgorithm.dfy"
+include "./trees/MerkleTrees.dfy"
+include "./algorithms/IndexBasedAlgorithm.dfy"
 
 /**
- *  A proof of correctness for the Deposit Smart Contract Algorith.
- *  Version using FP algorithm.
+ *  A proof of correctness for the Deposit Smart Contract Algorithm.
+ *  
  */
 module DepositSmart {
 
@@ -70,35 +70,22 @@ module DepositSmart {
         /** The list of values added so far. */
         ghost var values : seq<int> 
 
-        /** The (Merkle) tree that corresponds to the list of values added so far. */
-        ghost var t : Tree<int>
-
-        /** Path to index of next available leaf at index |values|. */
-        ghost var p : seq<bit>
 
         /** Property to maintain to ensure correctness. */
         predicate Valid()
             reads this
         {
             //  Height and sequences sizes.
-            1 <= TREE_HEIGHT ==  height(t) == |branch| == |zero_h| == |p|
+            1 <= TREE_HEIGHT == |branch| == |zero_h| 
             //  Maximum number of values stored in the tree bounded.
-            && count < power2(TREE_HEIGHT) == |leavesIn(t)|
+            && count < power2(TREE_HEIGHT) 
             //  count is the number of values added so far.
             && |values| == count
-            //  t is the Merkle tree for values. 
-            && isMerkle(t, values, f, d) && hasLeavesIndexedFrom(t, 0)
             //  zero_h is constant and equal to default values for each level of t.
             && zero_h == zeroes(f, d, TREE_HEIGHT - 1)
-            //  Left and right siblings of `p` are given by branch and zero_h.
-            //  p[i] == b means the sibling is at 1 - b, i.e. if p[i] == 0 (resp. 1), 
-            //  sibling is at level i is the right (resp. left) child. 
-            && (forall i :: 0 <= i < |p| ==> 
-                siblingValueAt(p, t, i + 1) == 
-                    if p[i] == 0 then zero_h[i] else branch[i]
-            )
-            //  `p` is the path to the next available slot in the tree at index `count`.
-            && p == natToBitList(count, TREE_HEIGHT)
+            //  branch and zero_h are the left and right siblings of path to 
+            //  |values|-th leaf in buildMerkle(values, TREE_HEIGHT, f, d)
+            && areSiblingsAtIndex(|values|, buildMerkle(values, TREE_HEIGHT, f, d), branch, zero_h)
         }
 
         /**
@@ -106,25 +93,29 @@ module DepositSmart {
          */
         constructor(h: nat, l : seq<int>, f1 : (int, int) -> int, default : int) 
             requires h >= 1
-            requires |l| == h && forall i :: 0 <= i < |l| ==> l[i] == 0
+            requires |l| == h 
             ensures Valid()
         {
             //  State variables
             TREE_HEIGHT, count, f, d := h, 0, f1, default;
-            branch, zero_h := l, zeroes(f1, default, h - 1);
+            zero_h, branch := zeroes(f1, default, h - 1), l ;
 
             //  Ghost variables
-            t, values, p := buildMerkle([], h, f1, default), [],  natToBitList(0, h);
+            values := [];
             
-            //  Proof that right siblings of p are zero_h.
+            //  Proof that right siblings of path atToBitList2(0, h) are zero_h.
             bitToNatToBitsIsIdentity(0, h);
             valueIsZeroImpliesAllZeroes(natToBitList2(0, h));
             leafAtPathIsIntValueOfPath(natToBitList2(0, h), buildMerkle([], h, f1, default), 0, 0);
             rightSiblingsOfLastPathAreDefault(natToBitList2(0, h), buildMerkle([], h, f1, default), 0, f1, 0, default);
         }
 
+        ///////////////////////////////////////////////////////////////////////////
+        //  Functional versions of algorithms.
+        ///////////////////////////////////////////////////////////////////////////
+
         /**
-         *  The (almost) function version deposit() function.
+         *  The (almost) functional version deposit() function.
          *
          *  This method updates the left siblings (branch) in order
          *  to maintain the correspondence with the Merkle tree for values.
@@ -140,66 +131,16 @@ module DepositSmart {
             ensures Valid()
             modifies this 
         {
-            ghost var nextTree :=  buildMerkle(values + [v], TREE_HEIGHT, f, d);
-            assert(p == natToBitList(|values|, TREE_HEIGHT));
-
-            //  Siblings of p in t are same as siblings on p in old(t)
-            forall (i : nat | 0 <= i < |p|)
-                ensures siblingValueAt(p, nextTree, i + 1) == 
-                     siblingValueAt(p, old(t), i + 1) ==
-                        if p[i] == 0 then
-                             zero_h[i]
-                        else 
-                            branch[i]
-            {
-                reveal_siblingValueAt();
-                nextPathSameSiblingsInNextList(
-                    TREE_HEIGHT, values, v, old(t), 
-                    nextTree, 
-                    f, d, p);
-            }
-            
-            bitToNatToBitsIsIdentity(count, TREE_HEIGHT);
-            pathToNoLasthasZero(p);
-            assert(exists i :: 0 <= i < |p| && p[i] == 0);
-
-            forall ( i : nat | 0 <= i < |nextPath(p)| && nextPath(p)[i] == 1)
-                ensures computeLeftSiblingOnNextPathFromLeftRight(p, branch, zero_h, f, v)[i]
-                    ==
-                    siblingValueAt(nextPath(p), nextTree, i + 1) 
-            {
-                computeLeftSiblingOnNextPathFromLeftRightIsCorrectInAMerkleTree(
-                    p, values, v, nextTree, branch, zero_h, f, d
-                );
-            }
-
-            pathToSucc(old(p), old(count), TREE_HEIGHT);
-            assert(nextPath(p) == natToBitList(old(count) + 1, TREE_HEIGHT));
-
-            ///////////////////////////////////////////////////////////////////
-            //  Compute new branch and increment count.
-            //  This is the actual algorithm.
-            ///////////////////////////////////////////////////////////////////
             branch := computeLeftSiblingsOnNextpathWithIndex(TREE_HEIGHT, count, branch, zero_h, f, v);
             count := count + 1;
-            ///////////////////////////////////////////////////////////////////
 
-            //  Update ghost vars
+             //  Update ghost vars and prove correctness with new tree
+            computeNewLeftIsCorrect(values, v, TREE_HEIGHT, old(branch), zero_h, f, d);
             values := values + [v];
-            p := nextPath(p);
-            t := buildMerkle(values, TREE_HEIGHT, f, d);
-            
-            pathToLastInMerkleTreeHasZeroRightSiblings(p, values, t, f, d);
-            forall (i : nat | 0 <= i < |p| && p[i] == 0 )
-                ensures siblingValueAt(p, t, i + 1) == zero_h[i]
-            {}
-            forall (i :nat | 0 <= i < |p| && p[i] == 1)
-                    ensures siblingValueAt(p, t, i + 1) == branch[i]
-            {}
         }   
 
         /**
-         *  The get_deposit_root() function.
+         *  The get_deposit_root() functional function.
          *
          *  This method should always return the root value of the tree.
          *
@@ -208,13 +149,185 @@ module DepositSmart {
         method get_deposit_root_f() returns (r : int) 
             requires Valid()
             ensures Valid()
-            /** The result is the root value of the tree.  */
-            ensures r == t.v 
+            /** The result is the root value of the tree that corresponds to `values`. */
+            ensures r == buildMerkle(values, TREE_HEIGHT, f, d).v 
         {
             r := computeRootLeftRightUpWithIndex(TREE_HEIGHT, count, branch, zero_h, f, d);
 
             //  The proof of post condition follows easily from:
-            computeRootUsingDefaultIsCorrectInAMerkleTree(p, values, t, branch, zero_h, f, d);
+            computeRootIsCorrect(values, TREE_HEIGHT, branch, zero_h, f, d);
+        }
+
+        ///////////////////////////////////////////////////////////////////////////
+        //  Imperative versions of algorithms.
+        ///////////////////////////////////////////////////////////////////////////
+
+        /** 
+         *  This method updates the left siblings (branch) in order
+         *  to maintain the correspondence with the Merkle tree for values.
+         *  This is captured by the Valid() predicate.
+         *  
+         *  @param  v   The new deposit amount.
+         */
+        method deposit(v : int) 
+            requires Valid()
+            requires count < power2(TREE_HEIGHT) - 1         
+            ensures Valid()
+            modifies this 
+        {
+            
+            var value := v;
+            var size : nat := count;
+            var i : nat := 0;
+            
+            ghost var e := computeLeftSiblingsOnNextpathWithIndex(TREE_HEIGHT, size, branch, zero_h, f, v);
+            ghost var p := natToBitList(|values|, TREE_HEIGHT);
+
+            assert(branch == take(branch, TREE_HEIGHT - i));
+            assert(zero_h == take(zero_h, TREE_HEIGHT - i));
+            assert(|e| == TREE_HEIGHT);
+            
+            ///////////////////////////////////////////////////////////////////
+            //  Compute new branch and increment count.
+            //  This is the actual algorithm.
+            ///////////////////////////////////////////////////////////////////
+            
+            while size % 2 == 1 
+                invariant zero_h == old(zero_h)  && p == old(p) && count == old(count) && values == old(values) && branch == old(branch)
+                invariant 0 <= TREE_HEIGHT - i - 1 
+                //  The next one is the important invariant that ensures
+                //  that the update of branch after the loop does not
+                //  result in a out of bounds error.
+                invariant TREE_HEIGHT - i - 1 < TREE_HEIGHT 
+                invariant |branch| == |e| == |zero_h| == TREE_HEIGHT
+                //  The sequel are helper invariants
+                invariant 0 <= size < power2(TREE_HEIGHT - i) - 1
+                invariant TREE_HEIGHT - i <= |p|
+                invariant |take(p, TREE_HEIGHT - i)| == TREE_HEIGHT - i
+                invariant size < power2(|take(p, TREE_HEIGHT - i)|)
+
+                // invariant 
+                invariant take(p, TREE_HEIGHT - i) == natToBitList2(size, TREE_HEIGHT - i)  // I1
+                invariant take(p, TREE_HEIGHT - i) == natToBitList2(size, |take(p, TREE_HEIGHT - i)|)  // I1
+                //  we have bot found a zero in p yet 
+
+                invariant e == 
+                    computeLeftSiblingsOnNextpathWithIndex(
+                        TREE_HEIGHT - i, size, 
+                        take(branch, TREE_HEIGHT - i), 
+                        take(zero_h, TREE_HEIGHT - i), f, value) 
+                    + drop(branch, TREE_HEIGHT - i);    //  proving the + may
+                    //  need sone help
+
+                //  Termination is easy as size decreases and must be zero.
+                decreases size 
+            {
+                //  Some help to verify I1:
+                div2IsInit(size, take(p, TREE_HEIGHT - i));
+                assert(size / 2 < power2(|take(p, TREE_HEIGHT - i - 1)|));
+                power2LessThanDiv2(size, TREE_HEIGHT - i);
+                // assert(size / 2 < power2(TREE_HEIGHT - i - 1) - 1);
+                assert(init(take(p, TREE_HEIGHT - i)) == take(p, TREE_HEIGHT - i - 1));
+
+                //  Some help to verify I2:
+                assert(init(take(branch, TREE_HEIGHT - i)) == take(branch, TREE_HEIGHT - i - 1));
+                assert(init(take(zero_h, TREE_HEIGHT - i)) == take(zero_h, TREE_HEIGHT - i - 1));
+                assert(last(take(branch, TREE_HEIGHT - i)) == branch[TREE_HEIGHT - i - 1]);
+
+                value := f(branch[TREE_HEIGHT - i - 1], value);
+                size := size / 2;
+                i := i + 1;
+            }
+            assert(count == old(count));
+            assert(e == computeLeftSiblingsOnNextpathWithIndex(
+                        TREE_HEIGHT - i, size, 
+                        take(branch, TREE_HEIGHT - i), 
+                        take(zero_h, TREE_HEIGHT - i), f, value) 
+                    + drop(branch, TREE_HEIGHT - i));
+            calc == {
+                e;
+                computeLeftSiblingsOnNextpathWithIndex(
+                        TREE_HEIGHT - i, size, 
+                        take(branch, TREE_HEIGHT - i), 
+                        take(zero_h, TREE_HEIGHT - i), f, value) 
+                    + drop(branch, TREE_HEIGHT - i);
+                { assert(size % 2 == 0); }
+                init(take(branch, TREE_HEIGHT - i)) + [value] + drop(branch, TREE_HEIGHT - i);
+                old(branch)[TREE_HEIGHT - i - 1 := value];
+            }
+            
+            //  This is the important hidden property: TREE_HEIGHT - i - 1 is NEVER 
+            //  out of range. 
+            branch := branch[TREE_HEIGHT - i - 1 := value];
+            assert(branch == old(branch)[TREE_HEIGHT - i - 1 := value]);
+            assert(branch == e);
+
+            count := count + 1;
+
+            //  Update ghost vars and prove correctness with new tree
+            computeNewLeftIsCorrect(values, v, TREE_HEIGHT, old(branch), zero_h, f, d);
+            values := values + [v];
+
+        }
+
+        /**
+         *  The get_deposit_root() function.
+         *
+         *  This method should always return the root value of the tree.
+         *
+         *  @returns    The root value of the Merkle Tree for values.
+         */
+         method get_deposit_root() returns (r : int) 
+            requires Valid()
+            ensures Valid()
+            /** The result of get_deposit_root_() is the root value of the tree.  */
+            ensures r == buildMerkle(values, TREE_HEIGHT, f, d).v 
+        {
+            //  Some help to prove that the main invariant holds on entry:
+            assert(take(branch, TREE_HEIGHT) == branch);
+            assert(take(zero_h, TREE_HEIGHT) == zero_h);
+
+            //  Store the expected result in a ghost variable.
+            ghost var e := computeRootLeftRightUpWithIndex(TREE_HEIGHT, count, branch, zero_h, f, d);
+
+            //  Start with default value for r.
+            r := d;
+            var h := 0;
+            var size := count;
+
+            while h < TREE_HEIGHT
+                //  no out of range in seqs:
+                invariant 0 <= h <= TREE_HEIGHT
+                invariant 0 <= size < power2(TREE_HEIGHT - h)
+                //  Main invariant:
+                invariant e == 
+                    computeRootLeftRightUpWithIndex(
+                        TREE_HEIGHT - h, size, 
+                        take(branch, TREE_HEIGHT - h), take(zero_h, TREE_HEIGHT - h), f, r)
+
+                decreases TREE_HEIGHT - h 
+            {
+                //  A little help for Dafny to check the proof:
+                assert(last(take(branch, TREE_HEIGHT - h)) == branch[TREE_HEIGHT - h - 1]);
+                assert(last(take(zero_h, TREE_HEIGHT - h)) == zero_h[TREE_HEIGHT - h - 1]);
+                assert(init(take(branch, TREE_HEIGHT - h)) == take(branch, TREE_HEIGHT - h - 1));
+                assert(init(take(zero_h, TREE_HEIGHT - h)) == take(zero_h, TREE_HEIGHT - h - 1));
+
+                if size % 2 == 1 {
+                    r := f(branch[TREE_HEIGHT - h - 1], r);
+                } else {
+                    r := f(r, zero_h[TREE_HEIGHT - h - 1]);
+                }
+                size := size / 2;
+                h := h + 1;
+            }
+
+            //  The correstness proof:
+            //  By invariant at the end of the loop and definition of computeRootLeftRightUpWithIndex
+            assert(e == computeRootLeftRightUpWithIndex(0, 0, [], [], f, r) == r);
+             //  The proof of post condition follows easily from:
+            computeRootIsCorrect(values, TREE_HEIGHT, branch, zero_h, f, d);
         }
     }
+   
 }
